working on some proofs.

theories/ExprDAs.v
@@ -37,14 +37,13 @@ Section parameterized.
   Qed.
 
   Lemma exprD'_typ0_weaken (ExprOk_expr : ExprOk _)
-  : forall (tus0 tvs0 : tenv typ) (l0 : expr)
-           (lD : exprT tus0 tvs0 T),
-      exprD'_typ0 tus0 tvs0 l0 = Some lD ->
-      forall tus' tvs' : list typ,
+  : forall (tus tvs tus' tvs' : tenv typ) (l0 : expr)
+           (lD : exprT tus tvs T),
+      exprD'_typ0 tus tvs l0 = Some lD ->
       exists
-        lD' : exprT (tus0 ++ tus') (tvs0 ++ tvs') T,
-        exprD'_typ0 (tus0 ++ tus') (tvs0 ++ tvs') l0 = Some lD' /\
-        (forall (us : hlist typD tus0) (vs : hlist typD tvs0)
+        lD' : exprT (tus ++ tus') (tvs ++ tvs') T,
+        exprD'_typ0 (tus ++ tus') (tvs ++ tvs') l0 = Some lD' /\
+        (forall (us : hlist typD tus) (vs : hlist typD tvs)
                 (us' : hlist typD tus') (vs' : hlist typD tvs'),
            lD us vs = lD' (hlist_app us us') (hlist_app vs vs')).
   Proof.
@@ -59,15 +58,14 @@ Section parameterized.
   Qed.
 
   Definition exprD'_typ0_weakenU (ExprOk_expr : ExprOk _)
-  : forall (tus0 tvs0 : tenv typ) (l0 : expr)
-           (lD : hlist typD tus0 -> hlist typD tvs0 -> T),
-      exprD'_typ0 tus0 tvs0 l0 = Some lD ->
-      forall tus' : list typ,
+  : forall (tus tvs tus' : tenv typ) (l0 : expr)
+           (lD : hlist typD tus -> hlist typD tvs -> T),
+      exprD'_typ0 tus tvs l0 = Some lD ->
       exists
-        lD' : hlist typD (tus0 ++ tus') -> hlist typD tvs0 -> T,
-        exprD'_typ0 (tus0 ++ tus') tvs0 l0 = Some lD' /\
-        (forall (us : hlist typD tus0) (us' : hlist typD tus')
-                (vs : hlist typD tvs0),
+        lD' : hlist typD (tus ++ tus') -> hlist typD tvs -> T,
+        exprD'_typ0 (tus ++ tus') tvs l0 = Some lD' /\
+        (forall (us : hlist typD tus) (us' : hlist typD tus')
+                (vs : hlist typD tvs),
            lD us vs = lD' (hlist_app us us') vs).
   Proof.
     unfold exprD'_typ0. intros.
@@ -83,14 +81,13 @@ Section parameterized.
   Qed.
 
   Definition exprD'_typ0_weakenV (ExprOk_expr : ExprOk _)
-  : forall (tus0 tvs0 : tenv typ) (l0 : expr)
-           (lD : hlist typD tus0 -> hlist typD tvs0 -> T),
-      exprD'_typ0 tus0 tvs0 l0 = Some lD ->
-      forall tvs' : list typ,
+  : forall (tus tvs tvs' : tenv typ) (l0 : expr)
+           (lD : hlist typD tus -> hlist typD tvs -> T),
+      exprD'_typ0 tus tvs l0 = Some lD ->
       exists
-        lD' : hlist typD tus0 -> hlist typD (tvs0 ++ tvs') -> T,
-        exprD'_typ0 tus0 (tvs0 ++ tvs') l0 = Some lD' /\
-        (forall (us : hlist typD tus0) (vs : hlist typD tvs0)
+        lD' : hlist typD tus -> hlist typD (tvs ++ tvs') -> T,
+        exprD'_typ0 tus (tvs ++ tvs') l0 = Some lD' /\
+        (forall (us : hlist typD tus) (vs : hlist typD tvs)
                 (vs' : hlist typD tvs'),
            lD us vs = lD' us (hlist_app vs vs')).
   Proof.
@@ -107,3 +104,7 @@ Section parameterized.
   Qed.
 
 End parameterized.
+
+Arguments exprD'_typ0_weakenU {_ _ _ _ _ _ _ tus tvs} tus' {_ _} _ : rename.
+Arguments exprD'_typ0_weakenV {_ _ _ _ _ _ _ tus tvs} tvs' {_ _} _ : rename.
+Arguments exprD'_typ0_weaken {_ _ _ _ _ _ _ tus tvs} tus' tvs' {_ _} _ : rename.
