theories/RTac/EApply.v
@@ -52,16 +52,9 @@ Section parameterized.
                      (GConj_list premises) (len_vars + nus) nvs
       end.
 
-  Let tyProp := @typ0 _ _ Prop _.
-
-  Let cast (e : typD tyProp) : Prop :=
-    match @typ0_cast typ _ Prop _ in _ = T return T with
-      | eq_refl => e
-    end.
-
   Hypothesis lemD :
-    @Lemma.lemmaD typ _ expr _ expr (@exprD'_typ0 _ _ _ _ Prop _)
-                  tyProp cast nil nil lem.
+    @Lemma.lemmaD typ expr _ _ expr (@exprD'_typ0 _ _ _ _ Prop _)
+                  _ nil nil lem.
 
   Theorem EAPPLY_sound : rtac_sound nil nil EAPPLY.
   Proof.
